Change isomorphism between per_elem (#81)
* [WIP] Change isomorphism between per_elem

* Change minor thing

* Finish change of basic lemmas

* Restore Realizability

* Improve proofs

* Restore all proofs

* Fix missing one as well

* Fix some proofs

* Add a pi case

* Add one more case

theories/Core/Semantic/PER/Definitions.v
@@ -8,41 +8,24 @@ Notation "'Dom' a ≈ b ∈ R" := ((R a b : Prop) : Prop) (in custom judg at lev
 Notation "'DF' a ≈ b ∈ R ↘ R'" := ((R R' a b : Prop) : Prop) (in custom judg at level 90, a custom domain, b custom domain, R constr, R' constr).
 Notation "'Exp' a ≈ b ∈ R" := (R a b : (Prop : Type)) (in custom judg at level 90, a custom exp, b custom exp, R constr).
 Notation "'EF' a ≈ b ∈ R ↘ R'" := (R R' a b : (Prop : Type)) (in custom judg at level 90, a custom exp, b custom exp, R constr, R' constr).
+(* Precedences of the next notations follow the ones in the standard library.
+   However, we do not use the ones in the standard library so that we can change
+   the relation if necessary in the future. *)
+Notation "R ~> R'" := (subrelation R R') (at level 70, right associativity).
+Notation "R <~> R'" := (relation_equivalence R R') (at level 95, no associativity).
 
 Generalizable All Variables.
 
 (** Helper Bundles *)
+(* Related modulo evaluation *)
 Inductive rel_mod_eval (R : relation domain -> domain -> domain -> Prop) A p A' p' R' : Prop := mk_rel_mod_eval : forall a a', {{ ⟦ A ⟧ p ↘ a }} -> {{ ⟦ A' ⟧ p' ↘ a' }} -> {{ DF a ≈ a' ∈ R ↘ R' }} -> rel_mod_eval R A p A' p' R'.
 #[global]
 Arguments mk_rel_mod_eval {_ _ _ _ _ _}.
 
-Inductive rel_mod_app (R : relation domain) f a f' a' : Prop := mk_rel_mod_app : forall fa f'a', {{ $| f & a |↘ fa }} -> {{ $| f' & a' |↘ f'a' }} -> {{ Dom fa ≈ f'a' ∈ R }} -> rel_mod_app R f a f' a'.
+(* Related modulo application *)
+Inductive rel_mod_app f a f' a' (R : relation domain) : Prop := mk_rel_mod_app : forall fa f'a', {{ $| f & a |↘ fa }} -> {{ $| f' & a' |↘ f'a' }} -> {{ Dom fa ≈ f'a' ∈ R }} -> rel_mod_app f a f' a' R.
 #[global]
 Arguments mk_rel_mod_app {_ _ _ _ _}.
-
-Ltac destruct_rel_by_assumption in_rel H :=
-  repeat
-    match goal with
-    | H' : {{ Dom ~?c ≈ ~?c' ∈ ?in_rel0 }} |- _ =>
-        tryif (unify in_rel0 in_rel)
-        then (destruct (H _ _ H') as []; destruct_all; mark_with H' 1)
-        else fail
-    end;
-  unmark_all_with 1.
-Ltac destruct_rel_mod_eval :=
-  repeat
-    match goal with
-    | H : (forall c c' (equiv_c_c' : {{ Dom c ≈ c' ∈ ?in_rel }}), rel_mod_eval _ _ _ _ _ _) |- _ =>
-        destruct_rel_by_assumption in_rel H; mark H
-    end;
-  unmark_all.
-Ltac destruct_rel_mod_app :=
-  repeat
-    match goal with
-    | H : (forall c c' (equiv_c_c' : {{ Dom c ≈ c' ∈ ?in_rel }}), rel_mod_app _ _ _ _ _) |- _ =>
-        destruct_rel_by_assumption in_rel H; mark H
-    end;
-  unmark_all.
 
 (** (Some Elements of) PER Lattice *)
 
@@ -83,56 +66,74 @@ Section Per_univ_elem_core_def.
 
   Inductive per_univ_elem_core : relation domain -> domain -> domain -> Prop :=
   | per_univ_elem_core_univ :
-    `{ forall (lt_j_i : j < i),
+    `{ forall (elem_rel : relation domain)
+          (lt_j_i : j < i),
           j = j' ->
-          {{ DF 𝕌@j ≈ 𝕌@j' ∈ per_univ_elem_core ↘ per_univ_rec lt_j_i }} }
-  | per_univ_elem_core_nat : {{ DF ℕ ≈ ℕ ∈ per_univ_elem_core ↘ per_nat }}
+          (elem_rel <~> per_univ_rec lt_j_i) ->
+          {{ DF 𝕌@j ≈ 𝕌@j' ∈ per_univ_elem_core ↘ elem_rel }} }
+  | per_univ_elem_core_nat :
+    forall (elem_rel : relation domain),
+      (elem_rel <~> per_nat) ->
+      {{ DF ℕ ≈ ℕ ∈ per_univ_elem_core ↘ elem_rel }}
   | per_univ_elem_core_pi :
     `{ forall (in_rel : relation domain)
          (out_rel : forall {c c'} (equiv_c_c' : {{ Dom c ≈ c' ∈ in_rel }}), relation domain)
+         (elem_rel : relation domain)
          (equiv_a_a' : {{ DF a ≈ a' ∈ per_univ_elem_core ↘ in_rel}}),
           PER in_rel ->
           (forall {c c'} (equiv_c_c' : {{ Dom c ≈ c' ∈ in_rel }}),
               rel_mod_eval per_univ_elem_core B d{{{ p ↦ c }}} B' d{{{ p' ↦ c' }}} (out_rel equiv_c_c')) ->
-          (forall f f', elem_rel f f' = forall {c c'} (equiv_c_c' : {{ Dom c ≈ c' ∈ in_rel }}), rel_mod_app (out_rel equiv_c_c') f c f' c') ->
+          (elem_rel <~> fun f f' => forall c c' (equiv_c_c' : {{ Dom c ≈ c' ∈ in_rel }}), rel_mod_app f c f' c' (out_rel equiv_c_c')) ->
           {{ DF Π a p B ≈ Π a' p' B' ∈ per_univ_elem_core ↘ elem_rel }} }
   | per_univ_elem_core_neut :
-    `{ {{ Dom b ≈ b' ∈ per_bot }} ->
-       {{ DF ⇑ a b ≈ ⇑ a' b' ∈ per_univ_elem_core ↘ per_ne }} }
+    `{ forall (elem_rel : relation domain),
+          {{ Dom b ≈ b' ∈ per_bot }} ->
+          (elem_rel <~> per_ne) ->
+          {{ DF ⇑ a b ≈ ⇑ a' b' ∈ per_univ_elem_core ↘ elem_rel }} }
   .
 
   Hypothesis
     (motive : relation domain -> domain -> domain -> Prop)
-      (case_U : forall (j j' : nat) (lt_j_i : j < i), j = j' -> motive (per_univ_rec lt_j_i) d{{{ 𝕌@j }}} d{{{ 𝕌@j' }}})
-      (case_nat : motive per_nat d{{{ ℕ }}} d{{{ ℕ }}})
+      (case_U : forall {j j' elem_rel} (lt_j_i : j < i),
+          j = j' ->
+          (elem_rel <~> per_univ_rec lt_j_i) ->
+          motive elem_rel d{{{ 𝕌@j }}} d{{{ 𝕌@j' }}})
+      (case_nat : forall {elem_rel},
+          (elem_rel <~> per_nat) ->
+          motive elem_rel d{{{ ℕ }}} d{{{ ℕ }}})
       (case_Pi :
-        forall {A p B A' p' B' in_rel elem_rel}
-           (out_rel : forall {c c'} (equiv_c_c' : {{ Dom c ≈ c' ∈ in_rel }}), relation domain),
+        forall {A p B A' p' B' in_rel}
+           (out_rel : forall {c c'} (equiv_c_c' : {{ Dom c ≈ c' ∈ in_rel }}), relation domain)
+           {elem_rel},
           {{ DF A ≈ A' ∈ per_univ_elem_core ↘ in_rel }} ->
           motive in_rel A A' ->
           PER in_rel ->
           (forall {c c'} (equiv_c_c' : {{ Dom c ≈ c' ∈ in_rel }}),
               rel_mod_eval (fun R x y => {{ DF x ≈ y ∈ per_univ_elem_core ↘ R }} /\ motive R x y) B d{{{ p ↦ c }}} B' d{{{ p' ↦ c' }}} (out_rel equiv_c_c')) ->
-          (forall f f', elem_rel f f' = forall {c c'} (equiv_c_c' : {{ Dom c ≈ c' ∈ in_rel }}), rel_mod_app (out_rel equiv_c_c') f c f' c') ->
+          (elem_rel <~> fun f f' => forall c c' (equiv_c_c' : {{ Dom c ≈ c' ∈ in_rel }}), rel_mod_app f c f' c' (out_rel equiv_c_c')) ->
           motive elem_rel d{{{ Π A p B }}} d{{{ Π A' p' B' }}})
-      (case_ne : (forall {a b a' b'}, {{ Dom b ≈ b' ∈ per_bot }} -> motive per_ne d{{{ ⇑ a b }}} d{{{ ⇑ a' b' }}})).
+      (case_ne : forall {a b a' b' elem_rel},
+          {{ Dom b ≈ b' ∈ per_bot }} ->
+          (elem_rel <~> per_ne) ->
+          motive elem_rel d{{{ ⇑ a b }}} d{{{ ⇑ a' b' }}}).
 
   #[derive(equations=no, eliminator=no)]
   Equations per_univ_elem_core_strong_ind R a b (H : {{ DF a ≈ b ∈ per_univ_elem_core ↘ R }}) : {{ DF a ≈ b ∈ motive ↘ R }} :=
-  | R, a, b, (per_univ_elem_core_univ lt_j_i eq)                         => case_U _ _ lt_j_i eq;
-  | R, a, b, per_univ_elem_core_nat                                      => case_nat;
-  | R, a, b, (per_univ_elem_core_pi in_rel out_rel equiv_a_a' per HT HE) =>
+  | R, a, b, (per_univ_elem_core_univ _ lt_j_i HE eq)                 => case_U lt_j_i HE eq;
+  | R, a, b, (per_univ_elem_core_nat _ HE)                            => case_nat HE;
+  | R, a, b, (per_univ_elem_core_pi _ out_rel _ equiv_a_a' per HT HE) =>
       case_Pi out_rel equiv_a_a' (per_univ_elem_core_strong_ind _ _ _ equiv_a_a') per
         (fun _ _ equiv_c_c' => match HT _ _ equiv_c_c' with
                               | mk_rel_mod_eval b b' evb evb' Rel =>
                                   mk_rel_mod_eval b b' evb evb' (conj _ (per_univ_elem_core_strong_ind _ _ _ Rel))
                               end)
         HE;
-  | R, a, b, (per_univ_elem_core_neut equiv_b_b')                        => case_ne equiv_b_b'.
+  | R, a, b, (per_univ_elem_core_neut _ equiv_b_b' HE)                => case_ne equiv_b_b' HE.
 
 End Per_univ_elem_core_def.
 
-Global Hint Constructors per_univ_elem_core : mcltt.
+#[export]
+Hint Constructors per_univ_elem_core : mcltt.
 
 Equations per_univ_elem (i : nat) : relation domain -> domain -> domain -> Prop by wf i :=
 | i => per_univ_elem_core i (fun j lt_j_i a a' => exists R', {{ DF a ≈ a' ∈ per_univ_elem j ↘ R' }}).
@@ -141,38 +142,47 @@ Definition per_univ (i : nat) : relation domain := fun a a' => exists R', {{ DF 
 #[global]
 Arguments per_univ _ _ _ /.
 
-Lemma per_univ_elem_core_univ' : forall j i,
+Lemma per_univ_elem_core_univ' : forall j i elem_rel,
     j < i ->
-    {{ DF 𝕌@j ≈ 𝕌@j ∈ per_univ_elem i ↘ per_univ j }}.
+    (elem_rel <~> per_univ j) ->
+    {{ DF 𝕌@j ≈ 𝕌@j ∈ per_univ_elem i ↘ elem_rel }}.
 Proof.
   intros.
   simp per_univ_elem.
-
-  eapply (per_univ_elem_core_univ i (fun j lt_j_i a a' => exists R', {{ DF a ≈ a' ∈ per_univ_elem j ↘ R' }}) H).
+  apply per_univ_elem_core_univ; try assumption.
   reflexivity.
 Qed.
-Global Hint Resolve per_univ_elem_core_univ' : mcltt.
+#[export]
+Hint Resolve per_univ_elem_core_univ' : mcltt.
 
 (** Universe/Element PER Induction Principle *)
 
 Section Per_univ_elem_ind_def.
   Hypothesis
     (motive : nat -> relation domain -> domain -> domain -> Prop)
-      (case_U : forall j j' i, j < i -> j = j' ->
-                           (forall A B R, {{ DF A ≈ B ∈ per_univ_elem j ↘ R }} -> motive j R A B) ->
-                           motive i (per_univ j) d{{{ 𝕌@j }}} d{{{ 𝕌@j' }}})
-      (case_N : forall i, motive i per_nat d{{{ ℕ }}} d{{{ ℕ }}})
+      (case_U : forall i {j j' elem_rel},
+          j < i -> j = j' ->
+          (elem_rel <~> per_univ j) ->
+          (forall A B R, {{ DF A ≈ B ∈ per_univ_elem j ↘ R }} -> motive j R A B) ->
+          motive i elem_rel d{{{ 𝕌@j }}} d{{{ 𝕌@j' }}})
+      (case_N : forall i {elem_rel},
+          (elem_rel <~> per_nat) ->
+          motive i elem_rel d{{{ ℕ }}} d{{{ ℕ }}})
       (case_Pi :
-        forall i {A p B A' p' B' in_rel elem_rel}
-           (out_rel : forall {c c'} (equiv_c_c' : {{ Dom c ≈ c' ∈ in_rel }}), relation domain),
+        forall i {A p B A' p' B' in_rel}
+           (out_rel : forall {c c'} (equiv_c_c' : {{ Dom c ≈ c' ∈ in_rel }}), relation domain)
+           {elem_rel},
           {{ DF A ≈ A' ∈ per_univ_elem i ↘ in_rel }} ->
           motive i in_rel A A' ->
           PER in_rel ->
           (forall {c c'} (equiv_c_c' : {{ Dom c ≈ c' ∈ in_rel }}),
               rel_mod_eval (fun R x y => {{ DF x ≈ y ∈ per_univ_elem i ↘ R }} /\ motive i R x y) B d{{{ p ↦ c }}} B' d{{{ p' ↦ c' }}} (out_rel equiv_c_c')) ->
-          (forall f f', elem_rel f f' = forall {c c'} (equiv_c_c' : {{ Dom c ≈ c' ∈ in_rel }}), rel_mod_app (out_rel equiv_c_c') f c f' c') ->
+          (elem_rel <~> fun f f' => forall c c' (equiv_c_c' : {{ Dom c ≈ c' ∈ in_rel }}), rel_mod_app f c f' c' (out_rel equiv_c_c')) ->
           motive i elem_rel d{{{ Π A p B }}} d{{{ Π A' p' B' }}})
-      (case_ne : (forall i {a b a' b'}, {{ Dom b ≈ b' ∈ per_bot }} -> motive i per_ne d{{{ ⇑ a b }}} d{{{ ⇑ a' b' }}})).
+      (case_ne : forall i {a b a' b' elem_rel},
+          {{ Dom b ≈ b' ∈ per_bot }} ->
+          (elem_rel <~> per_ne) ->
+          motive i elem_rel d{{{ ⇑ a b }}} d{{{ ⇑ a' b' }}}).
 
   #[local]
   Ltac def_simp := simp per_univ_elem in *.
@@ -182,50 +192,38 @@ Section Per_univ_elem_ind_def.
     (H : {{ DF a ≈ b ∈ per_univ_elem_core i (fun j lt_j_i a a' => exists R', {{ DF a ≈ a' ∈ per_univ_elem j ↘ R' }}) ↘ R }}) : {{ DF a ≈ b ∈ motive i ↘ R }} by wf i :=
   | i, R, a, b, H =>
       per_univ_elem_core_strong_ind i _ (motive i)
-        (fun j j' j_lt_i eq => case_U j j' i j_lt_i eq (fun A B R' H' => per_univ_elem_ind' _ R' A B _))
-        (case_N i)
-        (fun A p B A' p' B' in_rel elem_rel out_rel HA IHA per HT HE => case_Pi i out_rel _ IHA per _ HE)
-        (@case_ne i)
+        (fun _ _ _ j_lt_i eq HE => case_U i j_lt_i eq HE (fun A B R' H' => per_univ_elem_ind' _ R' A B _))
+        (fun _ => case_N i)
+        (fun _ _ _ _ _ _ _ out_rel _ _ IHA per _ => case_Pi i out_rel _ IHA per _)
+        (fun _ _ _ _ _ => case_ne i)
         R a b H.
 
   #[derive(equations=no, eliminator=no), tactic="def_simp"]
   Equations per_univ_elem_ind i a b R (H : per_univ_elem i a b R) : motive i a b R :=
   | i, a, b, R, H := per_univ_elem_ind' i a b R _.
-
 End Per_univ_elem_ind_def.
-
-(** Universe/Element PER Helper Tactics *)
-
-Ltac invert_per_univ_elem H :=
-  simp per_univ_elem in H;
-  inversion H;
-  subst;
-  try rewrite <- per_univ_elem_equation_1 in *.
-
-Ltac per_univ_elem_econstructor :=
-  simp per_univ_elem;
-  econstructor;
-  try rewrite <- per_univ_elem_equation_1 in *.
 
 (** Context/Environment PER *)
 
 Definition rel_typ (i : nat) (A : typ) (p : env) (A' : typ) (p' : env) R' := rel_mod_eval (per_univ_elem i) A p A' p' R'.
 Arguments rel_typ _ _ _ _ _ _ /.
 
-Definition per_total : relation env := fun p p' => True.
-
 Inductive per_ctx_env : relation env -> ctx -> ctx -> Prop :=
 | per_ctx_env_nil :
-  `{ {{ EF ⋅ ≈ ⋅ ∈ per_ctx_env ↘ per_total }} }
+  `{ forall env_rel,
+        (env_rel <~> fun p p' => True) ->
+        {{ EF ⋅ ≈ ⋅ ∈ per_ctx_env ↘ env_rel }} }
 | per_ctx_env_cons :
-  `{ forall (tail_rel : relation env)
+  `{ forall tail_rel
         (head_rel : forall {p p'} (equiv_p_p' : {{ Dom p ≈ p' ∈ tail_rel }}), relation domain)
+        env_rel
         (equiv_Γ_Γ' : {{ EF Γ ≈ Γ' ∈ per_ctx_env ↘ tail_rel }}),
         PER tail_rel ->
         (forall {p p'} (equiv_p_p' : {{ Dom p ≈ p' ∈ tail_rel }}),
             rel_typ i A p A' p' (head_rel equiv_p_p')) ->
-        (env_rel = fun p p' => exists (equiv_p_drop_p'_drop : {{ Dom p ↯ ≈ p' ↯ ∈ tail_rel }}),
-                       {{ Dom ~(p 0) ≈ ~(p' 0) ∈ head_rel equiv_p_drop_p'_drop }}) ->
+        (env_rel <~> fun p p' =>
+             exists (equiv_p_drop_p'_drop : {{ Dom p ↯ ≈ p' ↯ ∈ tail_rel }}),
+               {{ Dom ~(p 0) ≈ ~(p' 0) ∈ head_rel equiv_p_drop_p'_drop }}) ->
         {{ EF Γ, A ≈ Γ', A' ∈ per_ctx_env ↘ env_rel }} }
 .
 
