theories/Core/Completeness/FunctionCases.v
@@ -1,0 +1,139 @@
+From Coq Require Import Morphisms_Relations RelationClasses SetoidTactics.
+From Mcltt Require Import Base LibTactics LogicalRelation System.
+Import Domain_Notations.
+
+Lemma rel_exp_pi_cong : forall {i Γ A A' B B'},
+  {{ Γ ⊨ A ≈ A' : Type@i }} ->
+  {{ Γ , A ⊨ B ≈ B' : Type@i }} ->
+  {{ Γ ⊨ Π A B ≈ Π A' B' : Type@i }}.
+Proof.
+  pose proof (@relation_equivalence_pointwise domain).
+  pose proof (@relation_equivalence_pointwise env).
+  intros * [env_relΓ] [env_relΓA].
+  destruct_conjs.
+  pose (env_relΓ0 := env_relΓ).
+  pose (env_relΓA0 := env_relΓA).
+  inversion_by_head (per_ctx_env env_relΓA); subst.
+  handle_per_ctx_env_irrel.
+  eexists.
+  eexists; [eassumption |].
+  eexists.
+  intros.
+  (on_all_hyp: fun H => destruct_rel_by_assumption tail_rel H).
+  rewrite_relation_equivalence_right.
+  (on_all_hyp: fun H => destruct_rel_by_assumption env_relΓ H).
+  destruct_by_head rel_typ.
+  inversion_by_head (eval_exp {{{ Type@i }}}); subst.
+  match goal with
+  | H : per_univ_elem _ _ d{{{ 𝕌@?i }}} d{{{ 𝕌@?i }}} |- _ =>
+      invert_per_univ_elem H;
+      apply_relation_equivalence;
+      clear_refl_eqs
+  end.
+  destruct_by_head rel_exp.
+  destruct_conjs.
+  handle_per_univ_elem_irrel.
+  exists (per_univ i).
+  split; [> econstructor; only 1-2: repeat econstructor; eauto ..].
+  unfold per_univ.
+  eexists.
+  per_univ_elem_econstructor; try (now eauto); try setoid_reflexivity.
+  - eauto with typeclass_instances.
+  - instantiate (1 := fun c c' (equiv_c_c' : head_rel p p' equiv_p_p' c c') b b' =>
+                        forall a a' R,
+                          {{ ⟦ B ⟧ p ↦ c ↘ a }} ->
+                          {{ ⟦ B' ⟧ p' ↦ c' ↘ a' }} ->
+                          per_univ_elem i R a a' -> R b b').
+    intros.
+    assert (equiv_pc_p'c' : {{ Dom p ↦ c ≈ p' ↦ c' ∈ env_relΓA }}) by (apply_relation_equivalence; eexists; eauto).
+    apply_relation_equivalence.
+    (on_all_hyp: fun H => destruct (H _ _ equiv_pc_p'c') as [? []]).
+    destruct_by_head rel_typ.
+    destruct_by_head rel_exp.
+    inversion_by_head (eval_exp {{{ Type@i }}}).
+    subst.
+    match goal with
+    | H : per_univ_elem _ _ d{{{ 𝕌@?i }}} d{{{ 𝕌@?i }}} |- _ =>
+        invert_per_univ_elem H;
+        apply_relation_equivalence;
+        clear_refl_eqs
+    end.
+    destruct_conjs.
+    econstructor; mauto.
+    evar (elem_rel : relation domain).
+    match goal with
+    | |- per_univ_elem _ ?R _ _ => setoid_replace R with elem_rel; subst elem_rel; [eassumption |]
+    end.
+    split; intros; handle_per_univ_elem_irrel; intuition.
+  - match goal with
+    | |- ?X <~> ?Y => instantiate (1 := Y)
+    end.
+    reflexivity.
+Qed.      
+
+Lemma rel_exp_pi_sub : forall {i Γ σ Δ A B},
+    {{ Γ ⊨s σ : Δ }} ->
+    {{ Δ ⊨ A : Type@i }} ->
+    {{ Δ , A ⊨ B : Type@i }} ->
+    {{ Γ ⊨ (Π A B)[σ] ≈ Π (A[σ]) (B[q σ]) : Type@i }}.
+Proof.
+  pose proof (@relation_equivalence_pointwise domain).
+  pose proof (@relation_equivalence_pointwise env).
+  intros * [env_relΓ] [] [env_relΔA].
+  destruct_conjs.
+  pose (env_relΔA0 := env_relΔA).
+  inversion_by_head (per_ctx_env env_relΔA); subst.
+  handle_per_ctx_env_irrel.
+  eexists.
+  eexists; [eassumption |].
+  eexists.
+  intros.
+  (on_all_hyp: fun H => destruct_rel_by_assumption env_relΓ H).
+  (on_all_hyp: fun H => destruct_rel_by_assumption tail_rel H).
+  destruct_by_head rel_typ.
+  inversion_by_head (eval_exp {{{ Type@i }}}); subst.
+  match goal with
+  | H : per_univ_elem _ _ d{{{ 𝕌@?i }}} d{{{ 𝕌@?i }}} |- _ =>
+      invert_per_univ_elem H;
+      apply_relation_equivalence;
+      clear_refl_eqs
+  end.
+  destruct_by_head rel_exp.
+  destruct_conjs.
+  handle_per_univ_elem_irrel.
+  eexists; split;
+    [> econstructor; only 1-2: repeat econstructor; eauto ..].
+  eexists.
+  per_univ_elem_econstructor; eauto with typeclass_instances.
+  - instantiate (1 := fun c c' (equiv_c_c' : head_rel o o' H9 c c') b b' =>
+                        forall a a' R,
+                          {{ ⟦ B ⟧ o ↦ c ↘ a }} ->
+                          {{ ⟦ B[q σ] ⟧ p' ↦ c' ↘ a' }} ->
+                          per_univ_elem i R a a' -> R b b').
+    intros.
+    assert (equiv_pc_p'c' : {{ Dom o ↦ c ≈ o' ↦ c' ∈ env_relΔA }}) by (apply_relation_equivalence; eexists; eauto).
+    apply_relation_equivalence.
+    (on_all_hyp: fun H => destruct (H _ _ equiv_pc_p'c') as [? []]).
+    destruct_by_head rel_typ.
+    inversion_by_head (eval_exp {{{ Type@i }}}); subst.
+    match goal with
+    | H : per_univ_elem _ _ d{{{ 𝕌@?i }}} d{{{ 𝕌@?i }}} |- _ =>
+        invert_per_univ_elem H;
+        apply_relation_equivalence;
+        clear_refl_eqs
+    end.
+    destruct_by_head rel_exp.
+    destruct_conjs.
+    econstructor; only 1-2: repeat econstructor; eauto.
+    evar (elem_rel : relation domain).
+    match goal with
+    | |- per_univ_elem _ ?R _ _ => setoid_replace R with elem_rel; subst elem_rel; [eassumption |]
+    end.
+    split; intros; handle_per_univ_elem_irrel; intuition.
+    enough {{ ⟦ B[q σ] ⟧ p' ↦ c' ↘ m' }} by intuition.
+    repeat econstructor; eauto.
+  - match goal with
+    | |- ?X <~> ?Y => instantiate (1 := Y)
+    end.
+    reflexivity.
+Qed.
