theories/Core/Completeness/LogicalRelation/Definitions.v
@@ -1,0 +1,41 @@
+From Coq Require Import Relations.
+From Mcltt Require Import Base.
+From Mcltt Require Export Evaluation PER.
+Import Domain_Notations.
+
+Inductive rel_exp M p M' p' (R : relation domain) : Prop :=
+| mk_rel_exp : forall m m', {{ ⟦ M ⟧ p ↘ m }} -> {{ ⟦ M' ⟧ p' ↘ m' }} -> {{ Dom m ≈ m' ∈ R }} -> rel_exp M p M' p' R.
+#[global]
+Arguments mk_rel_exp {_ _ _ _ _}.
+
+Definition rel_exp_under_ctx Γ M M' A :=
+  exists env_rel (_ : {{ EF Γ ≈ Γ ∈ per_ctx_env ↘ env_rel }}) i,
+  forall p p' (equiv_p_p' : {{ Dom p ≈ p' ∈ env_rel }}),
+  exists (elem_rel : relation domain),
+     rel_typ i A p A p' elem_rel /\ rel_exp M p M' p' elem_rel.
+
+Definition valid_exp_under_ctx Γ M A := rel_exp_under_ctx Γ M M A.
+#[global]
+Arguments valid_exp_under_ctx _ _ _ /.
+
+Inductive rel_subst σ p σ' p' (R : relation env) : Prop :=
+| mk_rel_subst : forall o o', {{ ⟦ σ ⟧s p ↘ o }} -> {{ ⟦ σ' ⟧s p' ↘ o' }} -> {{ Dom o ≈ o' ∈ R }} -> rel_subst σ p σ' p' R.
+#[global]
+Arguments mk_rel_subst {_ _ _ _ _ _}.
+
+Definition rel_subst_under_ctx Γ σ σ' Δ :=
+  exists env_rel (_ : {{ EF Γ ≈ Γ ∈ per_ctx_env ↘ env_rel }})
+     env_rel' (_ : {{ EF Δ ≈ Δ ∈ per_ctx_env ↘ env_rel' }}),
+  forall p p' (equiv_p_p' : {{ Dom p ≈ p' ∈ env_rel }}),
+    rel_subst σ p σ' p' env_rel'.
+
+Definition valid_subst_under_ctx Γ σ Δ := rel_subst_under_ctx Γ σ σ Δ.
+#[global]
+Arguments valid_subst_under_ctx _ _ _ /.
+
+Notation "⊨ Γ ≈ Γ'" := (per_ctx Γ Γ')  (in custom judg at level 80, Γ custom exp, Γ' custom exp).
+Notation "⊨ Γ" := (valid_ctx Γ) (in custom judg at level 80, Γ custom exp).
+Notation "Γ ⊨ M ≈ M' : A" := (rel_exp_under_ctx Γ M M' A) (in custom judg at level 80, Γ custom exp, M custom exp, M' custom exp, A custom exp).
+Notation "Γ ⊨ M : A" := (valid_exp_under_ctx Γ M A) (in custom judg at level 80, Γ custom exp, M custom exp, A custom exp).
+Notation "Γ ⊨s σ ≈ σ' : Δ" := (rel_subst_under_ctx Γ σ σ' Δ) (in custom judg at level 80, Γ custom exp, σ custom exp, σ' custom exp, Δ custom exp).
+Notation "Γ ⊨s σ : Δ" := (valid_subst_under_ctx Γ σ Δ) (in custom judg at level 80, Γ custom exp, σ custom exp, Δ custom exp).
