theories/Core/Completeness/TermStructureCases.v
@@ -1,4 +1,4 @@
-From Coq Require Import Relations RelationClasses.
+From Coq Require Import Morphisms_Relations RelationClasses.
 From Mcltt Require Import Base LibTactics LogicalRelation System.
 Import Domain_Notations.
 
@@ -7,22 +7,25 @@ Lemma rel_exp_sub_cong : forall {Δ M M' A σ σ' Γ},
     {{ Γ ⊨s σ ≈ σ' : Δ }} ->
     {{ Γ ⊨ M[σ] ≈ M'[σ'] : A[σ] }}.
 Proof.
+  pose proof (@relation_equivalence_pointwise domain).
+  pose proof (@relation_equivalence_pointwise env).
   intros * [env_relΔ] [env_relΓ].
   destruct_conjs.
-  per_ctx_env_irrel_rewrite.
+  pose (env_relΔ0 := env_relΔ).
+  handle_per_ctx_env_irrel.
   eexists.
   eexists; try eassumption.
   eexists.
   intros.
-  assert (env_relΓ p' p) by (eapply per_env_sym; eauto).
-  assert (env_relΓ p p) by (eapply per_env_trans; eauto).
+  assert (env_relΓ p' p) by (symmetry; eauto).
+  assert (env_relΓ p p) by (etransitivity; eauto).
   (on_all_hyp: fun H => destruct_rel_by_assumption env_relΓ H).
-  per_univ_elem_irrel_rewrite.
-  assert (env_relΔ o o0) by (eapply per_env_trans; [eauto | | eapply per_env_sym]; revgoals; eauto).
+  handle_per_univ_elem_irrel.
+  assert (env_relΔ o o0) by (etransitivity; [|symmetry; intuition]; intuition).
   (on_all_hyp: fun H => destruct_rel_by_assumption env_relΔ H).
   destruct_by_head rel_exp.
   destruct_by_head rel_typ.
-  per_univ_elem_irrel_rewrite.
+  handle_per_univ_elem_irrel.
   eexists.
   split; [> econstructor; only 1-2: econstructor; eauto ..].
 Qed.
@@ -51,9 +54,13 @@ Lemma rel_exp_sub_compose : forall {Γ τ Γ' σ Γ'' M A},
     {{ Γ'' ⊨ M : A }} ->
     {{ Γ ⊨ M[σ ∘ τ] ≈ M[σ][τ] : A[σ ∘ τ] }}.
 Proof.
+  pose proof (@relation_equivalence_pointwise domain).
+  pose proof (@relation_equivalence_pointwise env).
   intros * [env_relΓ [? [env_relΓ']]] [? [? [env_relΓ'']]] [].
   destruct_conjs.
-  per_ctx_env_irrel_rewrite.
+  pose (env_relΓ'0 := env_relΓ').
+  pose (env_relΓ''0 := env_relΓ'').
+  handle_per_ctx_env_irrel.
   eexists.
   eexists; try eassumption.
   eexists.
@@ -61,15 +68,16 @@ Proof.
   assert (env_relΓ p' p) by (eapply per_env_sym; eauto).
   assert (env_relΓ p p) by (eapply per_env_trans; eauto).
   (on_all_hyp: fun H => destruct_rel_by_assumption env_relΓ H).
-  per_univ_elem_irrel_rewrite.
+  handle_per_univ_elem_irrel.
   (on_all_hyp: fun H => destruct_rel_by_assumption env_relΓ' H).
-  per_univ_elem_irrel_rewrite.
+  handle_per_univ_elem_irrel.
   (on_all_hyp: fun H => destruct_rel_by_assumption env_relΓ'' H).
+  handle_per_univ_elem_irrel.
   destruct_by_head rel_exp.
   destruct_by_head rel_typ.
-  per_univ_elem_irrel_rewrite.
+  handle_per_univ_elem_irrel.
   eexists.
-  split; [> econstructor; only 1-2: repeat econstructor; mauto ..].
+  split; [> econstructor; only 1-2: repeat econstructor; eauto ..].
 Qed.
 
 Lemma rel_exp_conv : forall {Γ M M' A A' i},
@@ -77,9 +85,12 @@ Lemma rel_exp_conv : forall {Γ M M' A A' i},
     {{ Γ ⊨ A ≈ A' : Type@i }} ->
     {{ Γ ⊨ M ≈ M' : A' }}.
 Proof.
+  pose proof (@relation_equivalence_pointwise domain).
+  pose proof (@relation_equivalence_pointwise env).
   intros * [env_relΓ] [env_relΓ'].
   destruct_conjs.
-  per_ctx_env_irrel_rewrite.
+  pose (env_relΓ0 := env_relΓ).
+  handle_per_ctx_env_irrel.
   eexists.
   eexists; try eassumption.
   eexists.
@@ -89,19 +100,26 @@ Proof.
   destruct_by_head rel_exp.
   destruct_by_head rel_typ.
   inversion_by_head (eval_exp {{{ Type@i }}}); subst.
-  per_univ_elem_irrel_rewrite.
-  match_by_head1 per_univ_elem ltac:(fun H => invert_per_univ_elem H; let n := numgoals in guard n <= 1); clear_refl_eqs.
+  handle_per_univ_elem_irrel.
+  match goal with
+  | H : per_univ_elem _ _ d{{{ 𝕌@?i }}} d{{{ 𝕌@?i }}} |- _ =>
+      invert_per_univ_elem H;
+      apply_relation_equivalence;
+      clear_refl_eqs
+  end.
   destruct_conjs.
-  per_univ_elem_irrel_rewrite.
+  handle_per_univ_elem_irrel.
   eexists.
   split; econstructor; eauto.
-  eapply per_univ_trans; [eapply per_univ_sym |]; eauto.
+  etransitivity; [symmetry |]; eauto.
 Qed.
 
 Lemma rel_exp_sym : forall {Γ M M' A},
     {{ Γ ⊨ M ≈ M' : A }} ->
     {{ Γ ⊨ M' ≈ M : A }}.
 Proof.
+  pose proof (@relation_equivalence_pointwise domain).
+  pose proof (@relation_equivalence_pointwise env).
   intros * [env_relΓ].
   destruct_conjs.
   econstructor.
@@ -112,7 +130,7 @@ Proof.
   (on_all_hyp: fun H => destruct_rel_by_assumption env_relΓ H); destruct_conjs.
   destruct_by_head rel_exp.
   destruct_by_head rel_typ.
-  per_univ_elem_irrel_rewrite.
+  handle_per_univ_elem_irrel.
   eexists.
   split; econstructor; eauto.
   eapply per_elem_sym; eauto.
@@ -123,20 +141,23 @@ Lemma rel_exp_trans : forall {Γ M1 M2 M3 A},
     {{ Γ ⊨ M2 ≈ M3 : A }} ->
     {{ Γ ⊨ M1 ≈ M3 : A }}.
 Proof.
+  pose proof (@relation_equivalence_pointwise domain).
+  pose proof (@relation_equivalence_pointwise env).
   intros * [env_relΓ] [env_relΓ'].
   destruct_conjs.
-  per_ctx_env_irrel_rewrite.
+  pose (env_relΓ0 := env_relΓ).
+  handle_per_ctx_env_irrel.
   econstructor.
   eexists; try eassumption.
   eexists.
   intros ? ? equiv_p_p'.
-  assert (env_relΓ p' p) by (eapply per_env_sym; eauto).
-  assert (env_relΓ p' p') by (eapply per_env_trans; eauto).
+  assert (env_relΓ p' p) by (symmetry; eauto).
+  assert (env_relΓ p' p') by (etransitivity; eauto).
   (on_all_hyp: fun H => destruct_rel_by_assumption env_relΓ H); destruct_conjs.
   destruct_by_head rel_exp.
   destruct_by_head rel_typ.
-  per_univ_elem_irrel_rewrite.
+  handle_per_univ_elem_irrel.
   eexists.
   split; econstructor; eauto.
-  eapply per_elem_trans; eauto.
+  etransitivity; eauto.
 Qed.
