theories/Core/Completeness/VariableCases.v
@@ -1,4 +1,4 @@
-From Coq Require Import Relations.
+From Coq Require Import Morphisms_Relations Relations.
 From Mcltt Require Import Base LibTactics LogicalRelation System.
 Import Domain_Notations.
 
@@ -8,15 +8,18 @@ Lemma valid_lookup : forall {Γ x A env_rel}
     exists i,
     forall p p' (equiv_p_p' : {{ Dom p ≈ p' ∈ env_rel }}),
     exists elem_rel,
-      rel_typ i A p A p' elem_rel /\ rel_exp elem_rel {{{ #x }}} p {{{ #x }}} p'.
+      rel_typ i A p A p' elem_rel /\ rel_exp {{{ #x }}} p {{{ #x }}} p' elem_rel.
 Proof with solve [repeat econstructor; mauto].
-  intros.
-  assert {{ #x : A ∈ Γ }} as HxinΓ by mauto.
-  remember Γ as Δ eqn:HΔΓ in HxinΓ, equiv_Γ_Γ at 2. clear HΔΓ. rename equiv_Γ_Γ into equiv_Γ_Δ.
-  remember A as A' eqn:HAA' in HxinΓ |- * at 2. clear HAA'.
+  pose proof (@relation_equivalence_pointwise domain).
+  pose proof (@relation_equivalence_pointwise env).
+  intros * ? HxinΓ.
+  assert {{ #x : A ∈ Γ }} as HxinΓ' by mauto.
+  remember Γ as Δ eqn:HΔΓ in HxinΓ', equiv_Γ_Γ at 2. clear HΔΓ. rename equiv_Γ_Γ into equiv_Γ_Δ.
+  remember A as A' eqn:HAA' in HxinΓ' |- * at 2. clear HAA'.
   gen Δ A' env_rel.
-  induction H; intros * equiv_Γ_Δ H0; inversion H0; subst; clear H0; inversion_clear equiv_Γ_Δ; subst;
-    try (specialize (IHctx_lookup _ _ _ equiv_Γ_Γ' H2) as [j ?]; destruct_conjs);
+  induction HxinΓ; intros * equiv_Γ_Δ HxinΓ0; inversion HxinΓ0; subst; clear HxinΓ0; inversion_clear equiv_Γ_Δ; subst;
+    [|specialize (IHHxinΓ _ _ _ equiv_Γ_Γ' H2) as [j ?]; destruct_conjs];
+    apply_relation_equivalence;
     eexists; intros ? ? [];
     (on_all_hyp: fun H => destruct_rel_by_assumption tail_rel H); destruct_conjs;
     eexists.
@@ -42,6 +45,8 @@ Lemma rel_exp_var_weaken : forall {Γ B x A},
     {{ #x : A ∈ Γ }} ->
     {{ Γ , B ⊨ #x[Wk] ≈ #(S x) : A[Wk] }}.
 Proof.
+  pose proof (@relation_equivalence_pointwise domain).
+  pose proof (@relation_equivalence_pointwise env).
   intros * [] HxinΓ.
   match_by_head1 per_ctx_env ltac:(fun H => inversion H); subst.
   unshelve epose proof (valid_lookup _ HxinΓ); revgoals; mauto.
@@ -49,6 +54,7 @@ Proof.
   eexists.
   eexists; try eassumption.
   eexists.
+  apply_relation_equivalence.
   intros ? ? [].
   (on_all_hyp: fun H => destruct_rel_by_assumption tail_rel H).
   destruct_by_head rel_typ.
