theories/Core/Semantic/PER/Lemmas.v
@@ -1,7 +1,35 @@
-From Coq Require Import Lia PeanoNat Relation_Definitions RelationClasses.
+From Coq Require Import Lia Morphisms Morphisms_Prop Morphisms_Relations PeanoNat Relation_Definitions RelationClasses.
 From Equations Require Import Equations.
-From Mcltt Require Import Axioms Base Evaluation LibTactics PER.Definitions Readback.
+From Mcltt Require Import Base Evaluation LibTactics PER.Definitions PER.CoreTactics Readback.
 Import Domain_Notations.
+
+Add Parametric Morphism A : (@all A)
+    with signature forall_relation (fun (x : A) => iff) ==> iff as all_iff_moprhism'.
+Proof.
+  unfold forall_relation.
+  split; intros ** ?; intuition.
+Qed.
+
+Add Parametric Morphism A : PER
+    with signature (@relation_equivalence A) ==> iff as PER_morphism.
+Proof.
+  split; intros []; econstructor; unfold Symmetric, Transitive in *; intuition.
+Qed.
+
+Add Parametric Morphism R0 `(R0_morphism : Proper _ ((@relation_equivalence domain) ==> (@relation_equivalence domain)) R0) A p A' p' : (rel_mod_eval R0 A p A' p')
+    with signature (@relation_equivalence domain) ==> iff as rel_mod_eval_morphism.
+Proof.
+  split; intros []; econstructor; try eassumption;
+    [> eapply R0_morphism; [symmetry + idtac |]; eassumption ..].
+Qed.
+
+Add Parametric Morphism f a f' a' : (rel_mod_app f a f' a')
+    with signature (@relation_equivalence domain) ==> iff as rel_mod_app_morphism.
+Proof.
+  intros * HRR'.
+  split; intros []; econstructor; try eassumption;
+    apply HRR'; eassumption.
+Qed.
 
 Lemma per_bot_sym : forall m n,
     {{ Dom m ≈ n ∈ per_bot }} ->
@@ -149,53 +177,118 @@ Qed.
 #[export]
 Hint Resolve per_ne_trans : mcltt.
 
-Lemma per_univ_elem_right_irrel : forall i i' R A B R' B',
-    per_univ_elem i R A B ->
-    per_univ_elem i' R' A B' ->
-    R = R'.
+Add Parametric Morphism i : (per_univ_elem i)
+    with signature (@relation_equivalence domain) ==> eq ==> eq ==> iff as per_univ_elem_morphism_iff.
 Proof with mautosolve.
+  simpl.
+  intros R R' HRR'.
+  split; intros Horig; [gen R' | gen R];
+    induction Horig using per_univ_elem_ind; per_univ_elem_econstructor; eauto;
+    try (etransitivity; [symmetry + idtac|]; eassumption);
+    intros;
+    destruct_rel_mod_eval;
+    econstructor...
+Qed.
+
+Add Parametric Morphism i : (per_univ_elem i)
+    with signature (@relation_equivalence domain) ==> (@relation_equivalence domain) as per_univ_elem_morphism_relation_equivalence.
+Proof with mautosolve.
+  intros ** a b.
+  simpl.
+  rewrite H.
+  reflexivity.
+Qed.
+
+Add Parametric Morphism i A p A' p' : (rel_typ i A p A' p')
+    with signature (@relation_equivalence domain) ==> iff as rel_typ_morphism.
+Proof.
+  intros * HRR'.
+  split; intros []; econstructor; try eassumption;
+    [setoid_rewrite <- HRR' | setoid_rewrite HRR']; eassumption.
+Qed.
+
+Ltac rewrite_relation_equivalence_left :=
+  repeat match goal with
+    | H : ?R1 <~> ?R2 |- _ =>
+        try setoid_rewrite H;
+        (on_all_hyp: fun H' => assert_fails (unify H H'); unmark H; setoid_rewrite H in H');
+        let T := type of H in
+        fold (id T) in H
+    end; unfold id in *.
+
+Ltac rewrite_relation_equivalence_right :=
+  repeat match goal with
+    | H : ?R1 <~> ?R2 |- _ =>
+        try setoid_rewrite H;
+        (on_all_hyp: fun H' => assert_fails (unify H H'); unmark H; setoid_rewrite <- H in H');
+        let T := type of H in
+        fold (id T) in H
+    end; unfold id in *.
+
+Ltac clear_relation_equivalence :=
+  repeat match goal with
+    | H : ?R1 <~> ?R2 |- _ =>
+        (unify R1 R2; clear H) + (is_var R1; clear R1 H) + (is_var R2; clear R2 H)
+    end.
+
+Ltac apply_relation_equivalence := rewrite_relation_equivalence_right; clear_relation_equivalence; rewrite_relation_equivalence_left; clear_relation_equivalence.
+
+Lemma per_univ_elem_right_irrel : forall i i' R a b R' b',
+    {{ DF a ≈ b ∈ per_univ_elem i ↘ R }} ->
+    {{ DF a ≈ b' ∈ per_univ_elem i' ↘ R' }} ->
+    (R <~> R').
+Proof with (destruct_rel_mod_eval; destruct_rel_mod_app; functional_eval_rewrite_clear; econstructor; intuition).
+  simpl.
   intros * Horig.
-  remember A as A' in |- *.
-  gen A' B' R'.
+  remember a as a' in |- *.
+  gen a' b' R'.
   induction Horig using per_univ_elem_ind; intros * Heq Hright;
     subst; invert_per_univ_elem Hright; unfold per_univ;
-    trivial.
+    intros;
+    apply_relation_equivalence;
+    try reflexivity.
   specialize (IHHorig _ _ _ eq_refl equiv_a_a').
-  subst.
-  extensionality f.
-  extensionality f'.
-  (on_all_hyp: fun H => rewrite H).
-  extensionality c.
-  extensionality c'.
-  extensionality equiv_c_c'.
-  destruct_rel_mod_eval.
-  functional_eval_rewrite_clear.
-  f_equal...
+  split; intros.
+  - rename equiv_c_c' into equiv0_c_c'.
+    assert (equiv_c_c' : in_rel c c') by firstorder...
+  - assert (equiv0_c_c' : in_rel0 c c') by firstorder...
 Qed.
 
 #[local]
-Ltac per_univ_elem_right_irrel_rewrite1 :=
+Ltac per_univ_elem_right_irrel_assert1 :=
   match goal with
-  | H1 : {{ DF ~?A ≈ ~?B ∈ per_univ_elem ?i ↘ ?R1 }}, H2 : {{ DF ~?A ≈ ~?B' ∈ per_univ_elem ?i ↘ ?R2 }} |- _ =>
-      clean replace R2 with R1 by first [solve [eauto using per_univ_elem_right_irrel] | fail 3]
+  | H1 : {{ DF ~?a ≈ ~?b ∈ per_univ_elem ?i ↘ ?R1 }},
+      H2 : {{ DF ~?a ≈ ~?b' ∈ per_univ_elem ?i' ↘ ?R2 }} |- _ =>
+      assert_fails (unify R1 R2);
+      match goal with
+      | H : R1 <~> R2 |- _ => fail 1
+      | H : R2 <~> R1 |- _ => fail 1
+      | _ => assert (R1 <~> R2) by (eapply per_univ_elem_right_irrel; [apply H1 | apply H2])
+      end
   end.
 #[local]
-Ltac per_univ_elem_right_irrel_rewrite := repeat per_univ_elem_right_irrel_rewrite1.  
+Ltac per_univ_elem_right_irrel_assert := repeat per_univ_elem_right_irrel_assert1.
 
-Lemma per_univ_elem_sym : forall i R A B,
-    per_univ_elem i R A B ->
-    per_univ_elem i R B A /\
-      (forall a b,
-          {{ Dom a ≈ b ∈ R }} ->
-          {{ Dom b ≈ a ∈ R }}).
-Proof with (try econstructor; mautosolve).
-  induction 1 using per_univ_elem_ind; subst.
+Lemma per_univ_elem_sym : forall i R a b,
+    {{ DF a ≈ b ∈ per_univ_elem i ↘ R }} ->
+    {{ DF b ≈ a ∈ per_univ_elem i ↘ R }} /\
+      (forall m m',
+          {{ Dom m ≈ m' ∈ R }} ->
+          {{ Dom m' ≈ m ∈ R }}).
+Proof with mautosolve.
+  simpl.
+  induction 1 using per_univ_elem_ind; subst;
+    (* why does rewrite on <~> works only with this? *)
+    pose proof (@relation_equivalence_pointwise domain).
   - split.
-    + apply per_univ_elem_core_univ'...
-    + intros * [? []%H1]...
-  - split...
+    + apply per_univ_elem_core_univ'; firstorder.
+    + intros.
+      rewrite H1 in *.
+      destruct_by_head per_univ.
+      eexists.
+      eapply proj1...
+  - split; [per_univ_elem_econstructor | intros; apply_relation_equivalence]...
   - destruct_conjs.
-    (on_all_hyp: fun H => setoid_rewrite H).
     split.
     + per_univ_elem_econstructor; eauto.
       intros.
@@ -203,76 +296,95 @@ Proof with (try econstructor; mautosolve).
       assert (in_rel c c) by (etransitivity; eassumption).
       destruct_rel_mod_eval.
       functional_eval_rewrite_clear.
-      per_univ_elem_right_irrel_rewrite...
-    + enough (forall a b : domain,
-                 (forall (c c' : domain) (equiv_c_c' : in_rel c c'), rel_mod_app (out_rel c c' equiv_c_c') a c b c') ->
-                 (forall (c c' : domain) (equiv_c_c' : in_rel c c'), rel_mod_app (out_rel c c' equiv_c_c') b c a c')) by eauto.
+      econstructor; mauto.
+      per_univ_elem_right_irrel_assert.
+      apply_relation_equivalence.
+      eassumption.
+    + apply_relation_equivalence.
       intros.
       assert (in_rel c' c) by eauto.
       assert (in_rel c c) by (etransitivity; eassumption).
       destruct_rel_mod_eval.
       destruct_rel_mod_app.
       functional_eval_rewrite_clear.
-      per_univ_elem_right_irrel_rewrite...
-  - split...
+      econstructor; mauto.
+      per_univ_elem_right_irrel_assert.
+      intuition.
+  - split; [econstructor | intros; apply_relation_equivalence]...
 Qed.
 
-Corollary per_univ_sym : forall i R A B,
-    per_univ_elem i R A B ->
-    per_univ_elem i R B A.
+Corollary per_univ_sym : forall i R a b,
+    {{ DF a ≈ b ∈ per_univ_elem i ↘ R }} ->
+    {{ DF b ≈ a ∈ per_univ_elem i ↘ R }}.
 Proof.
   intros * ?%per_univ_elem_sym.
   firstorder.
 Qed.
 
-Corollary per_elem_sym : forall i R A B a b,
-    per_univ_elem i R A B ->
-    R a b ->
-    R b a.
+Corollary per_elem_sym : forall i R a b m m',
+    {{ DF a ≈ b ∈ per_univ_elem i ↘ R }} ->
+    {{ Dom m ≈ m' ∈ R }} ->
+    {{ Dom m' ≈ m ∈ R }}.
 Proof.
   intros * ?%per_univ_elem_sym.
   firstorder.
 Qed.
 
-Corollary per_univ_elem_left_irrel : forall i i' R A B R' A',
-    per_univ_elem i R A B ->
-    per_univ_elem i' R' A' B ->
-    R = R'.
+Corollary per_univ_elem_left_irrel : forall i i' R a b R' a',
+    {{ DF a ≈ b ∈ per_univ_elem i ↘ R }} ->
+    {{ DF a' ≈ b ∈ per_univ_elem i' ↘ R' }} ->
+    (R <~> R').
 Proof.
   intros * ?%per_univ_sym ?%per_univ_sym.
   eauto using per_univ_elem_right_irrel.
 Qed.
 
-Corollary per_univ_elem_cross_irrel : forall i i' R A B R' B',
-    per_univ_elem i R A B ->
-    per_univ_elem i' R' B' A ->
-    R = R'.
+Corollary per_univ_elem_cross_irrel : forall i i' R a b R' b',
+    {{ DF a ≈ b ∈ per_univ_elem i ↘ R }} ->
+    {{ DF b' ≈ a ∈ per_univ_elem i' ↘ R' }} ->
+    (R <~> R').
 Proof.
   intros * ? ?%per_univ_sym.
   eauto using per_univ_elem_right_irrel.
 Qed.
 
-Ltac do_per_univ_elem_irrel_rewrite1 :=
-  let tactic_error o1 o2 := fail 3 "per_univ_elem_irrel equality between" o1 "and" o2 "cannot be solved by eauto" in
+Ltac do_per_univ_elem_irrel_assert1 :=
+  let tactic_error o1 o2 := fail 2 "per_univ_elem_irrel biconditional between" o1 "and" o2 "cannot be solved" in
   match goal with
-    | H1 : {{ DF ~?A ≈ ~_ ∈ per_univ_elem ?i ↘ ?R1 }},
-        H2 : {{ DF ~?A ≈ ~_ ∈ per_univ_elem ?i' ↘ ?R2 }} |- _ =>
-        clean replace R2 with R1 by first [solve [eauto using per_univ_elem_right_irrel] | tactic_error R2 R1]
-    | H1 : {{ DF ~_ ≈ ~?B ∈ per_univ_elem ?i ↘ ?R1 }},
-        H2 : {{ DF ~_ ≈ ~?B ∈ per_univ_elem ?i' ↘ ?R2 }} |- _ =>
-        clean replace R2 with R1 by first [solve [eauto using per_univ_elem_left_irrel] | tactic_error R2 R1]
-    | H1 : {{ DF ~?A ≈ ~_ ∈ per_univ_elem ?i ↘ ?R1 }},
-        H2 : {{ DF ~_ ≈ ~?A ∈ per_univ_elem ?i' ↘ ?R2 }} |- _ =>
-        (* Order matters less here as H1 and H2 cannot be exchanged *)
-        clean replace R2 with R1 by first [solve [symmetry; eauto using per_univ_elem_cross_irrel] | tactic_error R2 R1]
-    end.
+  | H1 : {{ DF ~?A ≈ ~_ ∈ per_univ_elem ?i ↘ ?R1 }},
+      H2 : {{ DF ~?A ≈ ~_ ∈ per_univ_elem ?i' ↘ ?R2 }} |- _ =>
+      assert_fails (unify R1 R2);
+      match goal with
+      | H : R1 <~> R2 |- _ => fail 1
+      | H : R2 <~> R1 |- _ => fail 1
+      | _ => assert (R1 <~> R2) by (eapply per_univ_elem_right_irrel; [apply H1 | apply H2]) || tactic_error R1 R2
+      end
+  | H1 : {{ DF ~_ ≈ ~?B ∈ per_univ_elem ?i ↘ ?R1 }},
+      H2 : {{ DF ~_ ≈ ~?B ∈ per_univ_elem ?i' ↘ ?R2 }} |- _ =>
+      assert_fails (unify R1 R2);
+      match goal with
+      | H : R1 <~> R2 |- _ => fail 1
+      | H : R2 <~> R1 |- _ => fail 1
+      | _ => assert (R1 <~> R2) by (eapply per_univ_elem_left_irrel; [apply H1 | apply H2]) || tactic_error R1 R2
+      end
+  | H1 : {{ DF ~?A ≈ ~_ ∈ per_univ_elem ?i ↘ ?R1 }},
+      H2 : {{ DF ~_ ≈ ~?A ∈ per_univ_elem ?i' ↘ ?R2 }} |- _ =>
+      (* Order matters less here as H1 and H2 cannot be exchanged *)
+      assert_fails (unify R1 R2);
+      match goal with
+      | H : R1 <~> R2 |- _ => fail 1
+      | H : R2 <~> R1 |- _ => fail 1
+      | _ => assert (R1 <~> R2) by (eapply per_univ_elem_cross_irrel; [apply H1 | apply H2]) || tactic_error R1 R2
+      end
+  end.
 
-Ltac do_per_univ_elem_irrel_rewrite :=
-  repeat do_per_univ_elem_irrel_rewrite1.
+Ltac do_per_univ_elem_irrel_assert :=
+  repeat do_per_univ_elem_irrel_assert1.
 
-Ltac per_univ_elem_irrel_rewrite :=
+Ltac handle_per_univ_elem_irrel :=
   functional_eval_rewrite_clear;
-  do_per_univ_elem_irrel_rewrite;
+  do_per_univ_elem_irrel_assert;
+  apply_relation_equivalence;
   clear_dups.
 
 Lemma per_univ_elem_trans : forall i R A1 A2,
@@ -284,32 +396,45 @@ Lemma per_univ_elem_trans : forall i R A1 A2,
           R a1 a2 ->
           R a2 a3 ->
           R a1 a3).
-Proof with ((econstructor + per_univ_elem_econstructor); mautosolve).
+Proof with (per_univ_elem_econstructor; mautosolve).
+  pose proof (@relation_equivalence_pointwise domain).
   induction 1 using per_univ_elem_ind;
     [> split;
      [ intros * HT2; invert_per_univ_elem HT2; clear HT2
-     | intros * HTR1 HTR2 ] ..]; mauto.
-  - destruct HTR1, HTR2.
-    per_univ_elem_irrel_rewrite.
-    specialize (H1 _ _ _ H2) as [].
-    specialize (H0 _ _ H3)...
-  - idtac...
-  - per_univ_elem_irrel_rewrite.
-    rename in_rel0 into in_rel.
-    destruct IHper_univ_elem as [].
+     | intros * HTR1 HTR2; apply_relation_equivalence ] ..]; mauto.
+  - (* univ case *)
+    subst.
+    destruct HTR1, HTR2.
+    functional_eval_rewrite_clear.
+    handle_per_univ_elem_irrel.
+    specialize (H3 _ _ _ H1) as [].
+    eexists.
+    intuition.
+  - (* nat case *)
+    idtac...
+  - (* pi case *)
+    destruct_conjs.
     per_univ_elem_econstructor; eauto.
+    + handle_per_univ_elem_irrel.
+      intuition.
+    + intros.
+      handle_per_univ_elem_irrel.
+      assert (in_rel c c') by firstorder.
+      assert (in_rel c c) by intuition.
+      assert (in_rel0 c c) by intuition.
+      destruct_rel_mod_eval.
+      functional_eval_rewrite_clear.
+      handle_per_univ_elem_irrel...
+  - (* fun case *)
     intros.
-    assert (in_rel c c) by (etransitivity; [ | symmetry]; eassumption).
-    destruct_rel_mod_eval.
-    per_univ_elem_irrel_rewrite...
-  - destruct IHper_univ_elem as [].
-    rewrite H2 in *.
-    intros.
-    assert (in_rel c' c') by (etransitivity; [symmetry | ]; eassumption).
+    assert (in_rel c c) by intuition.
     destruct_rel_mod_eval.
     destruct_rel_mod_app.
-    per_univ_elem_irrel_rewrite...
-  - idtac...
+    handle_per_univ_elem_irrel.
+    econstructor; eauto.
+    intuition.
+  - (* neut case *)
+    idtac...
 Qed.
 
 Corollary per_univ_trans : forall i j R A1 A2 A3,
@@ -331,22 +456,20 @@ Proof.
   firstorder.
 Qed.
 
-
 #[export]
-  Instance per_elem_PER {i R A B} `(H : per_univ_elem i R A B) : PER R.
-Proof.
-  split.
-  - auto using (per_elem_sym _ _ _ _ _ _ H).
-  - eauto using (per_elem_trans _ _ _ _ _ _ _ H).
-Qed.
-
-
-#[export]
-  Instance per_univ_PER {i R} : PER (per_univ_elem i R).
+Instance per_univ_PER {i R} : PER (per_univ_elem i R).
 Proof.
   split.
   - auto using per_univ_sym.
   - eauto using per_univ_trans.
+Qed.
+
+#[export]
+Instance per_elem_PER {i R A B} `(H : per_univ_elem i R A B) : PER R.
+Proof.
+  split.
+  - eauto using (per_elem_sym _ _ _ _ _ _ H).
+  - eauto using (per_elem_trans _ _ _ _ _ _ _ H).
 Qed.
 
 (* This lemma gets rid of the unnecessary PER premise. *)
@@ -357,14 +480,13 @@ Lemma per_univ_elem_core_pi' :
     (equiv_a_a' : {{ DF A ≈ A' ∈ per_univ_elem i ↘ in_rel}}),
     (forall {c c'} (equiv_c_c' : {{ Dom c ≈ c' ∈ in_rel }}),
         rel_mod_eval (per_univ_elem i) B d{{{ p ↦ c }}} B' d{{{ p' ↦ c' }}} (out_rel equiv_c_c')) ->
-    (forall f f', elem_rel f f' = forall {c c'} (equiv_c_c' : {{ Dom c ≈ c' ∈ in_rel }}), rel_mod_app (out_rel equiv_c_c') f c f' c') ->
+    (elem_rel <~> fun f f' => forall c c' (equiv_c_c' : {{ Dom c ≈ c' ∈ in_rel }}), rel_mod_app f c f' c' (out_rel equiv_c_c')) ->
     {{ DF Π A p B ≈ Π A' p' B' ∈ per_univ_elem i ↘ elem_rel }}.
 Proof.
   intros.
   per_univ_elem_econstructor; eauto.
   typeclasses eauto.
 Qed.
-
 
 Lemma per_univ_elem_cumu : forall i a0 a1 R,
     {{ DF a0 ≈ a1 ∈ per_univ_elem i ↘ R }} ->
@@ -373,7 +495,7 @@ Proof with solve [eauto].
   simpl.
   induction 1 using per_univ_elem_ind; subst.
   - eapply per_univ_elem_core_univ'...
-  - per_univ_elem_econstructor.
+  - per_univ_elem_econstructor...
   - per_univ_elem_econstructor; mauto.
     intros.
     destruct_rel_mod_eval.
@@ -381,24 +503,39 @@ Proof with solve [eauto].
   - per_univ_elem_econstructor...
 Qed.
 
+Add Parametric Morphism : per_ctx_env
+    with signature (@relation_equivalence env) ==> eq ==> eq ==> iff as per_ctx_env_morphism_iff.
+Proof with mautosolve.
+  intros R R' HRR'.
+  split; intro Horig; [gen R' | gen R];
+    induction Horig; econstructor;
+    apply_relation_equivalence; try reflexivity...
+Qed.
+
+Add Parametric Morphism : per_ctx_env
+    with signature (@relation_equivalence env) ==> (@relation_equivalence ctx) as per_ctx_env_morphism_relation_equivalence.
+Proof with mautosolve.
+  intros * HRR' Γ Γ'.
+  simpl.
+  rewrite HRR'.
+  reflexivity.
+Qed.
+
 Lemma per_ctx_env_right_irrel : forall Γ Δ Δ' R R',
     {{ DF Γ ≈ Δ ∈ per_ctx_env ↘ R }} ->
     {{ DF Γ ≈ Δ' ∈ per_ctx_env ↘ R' }} ->
-    R = R'.
-Proof.
+    R <~> R'.
+Proof with (destruct_rel_typ; handle_per_univ_elem_irrel; eexists; intuition).
   intros * Horig; gen Δ' R'.
   induction Horig; intros * Hright;
-    inversion Hright; subst; try congruence.
+    inversion Hright; subst;
+    apply_relation_equivalence;
+    try reflexivity.
   specialize (IHHorig _ _ equiv_Γ_Γ'0).
-  subst.
-  enough (head_rel = head_rel0) by now subst.
-  extensionality p.
-  extensionality p'.
-  extensionality equiv_p_p'.
-  simpl in *.
-  destruct_rel_mod_eval.
-  per_univ_elem_irrel_rewrite.
-  congruence.
+  intros p p'.
+  split; intros [].
+  - assert (equiv0_p_drop_p'_drop : {{ Dom p ↯ ≈ p' ↯ ∈ tail_rel0 }}) by intuition...
+  - assert (equiv_p_drop_p'_drop : {{ Dom p ↯ ≈ p' ↯ ∈ tail_rel }}) by intuition...
 Qed.
 
 Lemma per_ctx_env_sym : forall Γ Δ R,
@@ -407,25 +544,23 @@ Lemma per_ctx_env_sym : forall Γ Δ R,
       (forall o p,
           {{ Dom o ≈ p ∈ R }} ->
           {{ Dom p ≈ o ∈ R }}).
-Proof with solve [eauto using per_univ_sym].
+Proof with solve [intuition].
   simpl.
-  induction 1; split; try solve [econstructor; eauto]; simpl in *; destruct_conjs.
-  - econstructor; eauto.
-    intros.
-    assert (tail_rel p' p) by eauto.
-    assert (tail_rel p p) by (etransitivity; eauto).
+  induction 1; split; simpl in *; destruct_conjs; try econstructor; intuition;
+    pose proof (@relation_equivalence_pointwise env).
+  - assert (tail_rel p' p) by eauto.
+    assert (tail_rel p p) by (etransitivity; eassumption).
     destruct_rel_mod_eval.
-    per_univ_elem_irrel_rewrite.
-    econstructor...
-  - subst.
-    intros.
+    handle_per_univ_elem_irrel.
+    econstructor; eauto.
+    symmetry...
+  - apply_relation_equivalence.
     destruct_conjs.
     assert (tail_rel d{{{ p ↯ }}} d{{{ o ↯ }}}) by eauto.
-    assert (tail_rel d{{{ p ↯ }}} d{{{ p ↯ }}}) by (etransitivity; eauto).
+    assert (tail_rel d{{{ p ↯ }}} d{{{ p ↯ }}}) by (etransitivity; eassumption).
     destruct_rel_mod_eval.
     eexists.
-    per_univ_elem_irrel_rewrite.
-    eapply per_elem_sym...
+    handle_per_univ_elem_irrel; symmetry; intuition.
 Qed.
 
 Corollary per_ctx_sym : forall Γ Δ R,
@@ -448,7 +583,7 @@ Qed.
 Corollary per_ctx_env_left_irrel : forall Γ Γ' Δ R R',
     {{ DF Γ ≈ Δ ∈ per_ctx_env ↘ R }} ->
     {{ DF Γ' ≈ Δ ∈ per_ctx_env ↘ R' }} ->
-    R = R'.
+    R <~> R'.
 Proof.
   intros * ?%per_ctx_sym ?%per_ctx_sym.
   eauto using per_ctx_env_right_irrel.
@@ -457,33 +592,49 @@ Qed.
 Corollary per_ctx_env_cross_irrel : forall Γ Δ Δ' R R',
     {{ DF Γ ≈ Δ ∈ per_ctx_env ↘ R }} ->
     {{ DF Δ' ≈ Γ ∈ per_ctx_env ↘ R' }} ->
-    R = R'.
+    R <~> R'.
 Proof.
   intros * ? ?%per_ctx_sym.
   eauto using per_ctx_env_right_irrel.
 Qed.
 
-Ltac do_per_ctx_env_irrel_rewrite1 :=
+Ltac do_per_ctx_env_irrel_assert1 :=
   let tactic_error o1 o2 := fail 3 "per_ctx_env_irrel equality between" o1 "and" o2 "cannot be solved by mauto" in
   match goal with
     | H1 : {{ DF ~?Γ ≈ ~_ ∈ per_ctx_env ↘ ?R1 }},
         H2 : {{ DF ~?Γ ≈ ~_ ∈ per_ctx_env ↘ ?R2 }} |- _ =>
-        clean replace R2 with R1 by first [solve [eauto using per_ctx_env_right_irrel] | tactic_error R2 R1]
+        assert_fails (unify R1 R2);
+        match goal with
+        | H : R1 <~> R2 |- _ => fail 1
+        | H : R2 <~> R1 |- _ => fail 1
+        | _ => assert (R1 <~> R2) by (eapply per_ctx_env_right_irrel; [apply H1 | apply H2]) || tactic_error R1 R2
+        end
     | H1 : {{ DF ~_ ≈ ~?Δ ∈ per_ctx_env ↘ ?R1 }},
         H2 : {{ DF ~_ ≈ ~?Δ ∈ per_ctx_env ↘ ?R2 }} |- _ =>
-        clean replace R2 with R1 by first [solve [eauto using per_ctx_env_left_irrel] | tactic_error R2 R1]
+        assert_fails (unify R1 R2);
+        match goal with
+        | H : R1 <~> R2 |- _ => fail 1
+        | H : R2 <~> R1 |- _ => fail 1
+        | _ => assert (R1 <~> R2) by (eapply per_ctx_env_left_irrel; [apply H1 | apply H2]) || tactic_error R1 R2
+        end
     | H1 : {{ DF ~?Γ ≈ ~_ ∈ per_ctx_env ↘ ?R1 }},
         H2 : {{ DF ~_ ≈ ~?Γ ∈ per_ctx_env ↘ ?R2 }} |- _ =>
         (* Order matters less here as H1 and H2 cannot be exchanged *)
-        clean replace R2 with R1 by first [solve [symmetry; eauto using per_ctx_env_cross_irrel] | tactic_error R2 R1]
+        assert_fails (unify R1 R2);
+        match goal with
+        | H : R1 <~> R2 |- _ => fail 1
+        | H : R2 <~> R1 |- _ => fail 1
+        | _ => assert (R1 <~> R2) by (eapply per_ctx_env_cross_irrel; [apply H1 | apply H2]) || tactic_error R1 R2
+        end
     end.
 
-Ltac do_per_ctx_env_irrel_rewrite :=
-  repeat do_per_ctx_env_irrel_rewrite1.
+Ltac do_per_ctx_env_irrel_assert :=
+  repeat do_per_ctx_env_irrel_assert1.
 
-Ltac per_ctx_env_irrel_rewrite :=
+Ltac handle_per_ctx_env_irrel :=
   functional_eval_rewrite_clear;
-  do_per_ctx_env_irrel_rewrite;
+  do_per_ctx_env_irrel_assert;
+  apply_relation_equivalence;
   clear_dups.
 
 Lemma per_ctx_env_trans : forall Γ1 Γ2 R,
@@ -500,21 +651,27 @@ Proof with solve [eauto using per_univ_trans].
   induction 1; subst;
     [> split;
      [ inversion 1; subst; eauto
-     | intros; destruct_conjs; unfold per_total; eauto] ..];
-    per_ctx_env_irrel_rewrite.
-  - rename tail_rel0 into tail_rel.
-    econstructor; eauto.
-    + eapply IHper_ctx_env...
+     | intros; destruct_conjs; eauto] ..];
+    pose proof (@relation_equivalence_pointwise env);
+    handle_per_ctx_env_irrel;
+    try solve [intuition].
+  - econstructor; only 4: reflexivity; eauto.
+    + apply_relation_equivalence. intuition.
     + intros.
-      assert (tail_rel p p) by (etransitivity; [| symmetry]; eauto).
-      (on_all_hyp: fun H => destruct_rel_by_assumption tail_rel H).
-      per_univ_elem_irrel_rewrite.
-      econstructor...
-  - assert (tail_rel d{{{ p1 ↯ }}} d{{{ p3 ↯ }}}) by mauto.
+      assert (tail_rel p p) by intuition.
+      assert (tail_rel0 p p') by intuition.
+      destruct_rel_typ.
+      handle_per_univ_elem_irrel.
+      econstructor; intuition.
+      (* This one cannot be replaced with `etransitivity` as we need different `i`s. *)
+      eapply per_univ_trans; [| eassumption]; eassumption.
+  - destruct_conjs.
+    assert (tail_rel d{{{ p1 ↯ }}} d{{{ p3 ↯ }}}) by eauto.
+    destruct_rel_typ.
+    handle_per_univ_elem_irrel.
     eexists.
-    (on_all_hyp: fun H => destruct_rel_by_assumption tail_rel H).
-    per_univ_elem_irrel_rewrite.
-    eapply per_elem_trans...
+    apply_relation_equivalence.
+    etransitivity; intuition.
 Qed.
 
 Corollary per_ctx_trans : forall Γ1 Γ2 Γ3 R,
@@ -536,18 +693,16 @@ Proof.
   firstorder.
 Qed.
 
-
 #[export]
-  Instance per_ctx_PER {R} : PER (per_ctx_env R).
+Instance per_ctx_PER {R} : PER (per_ctx_env R).
 Proof.
   split.
   - auto using per_ctx_sym.
   - eauto using per_ctx_trans.
 Qed.
 
-
 #[export]
-  Instance per_env_PER {R Γ Δ} (H : per_ctx_env R Γ Δ) : PER R.
+Instance per_env_PER {R Γ Δ} (H : per_ctx_env R Γ Δ) : PER R.
 Proof.
   split.
   - auto using (per_env_sym _ _ _ _ _ H).
